Add the configuration requirements in the precondition of create_in_stack (no dynamic check)

providers/evercrypt/fst/EverCrypt.AEAD.fst
@@ -69,12 +69,11 @@ let invariant_s #a h (Ek i kv ek) =
   B.live h ek /\
   B.length ek >= concrete_xkey_length i /\
   B.as_seq h (B.gsub ek 0ul (UInt32.uint_to_t (concrete_xkey_length i)))
-    `S.equal` concrete_expand i (G.reveal kv) /\ (
+    `S.equal` concrete_expand i (G.reveal kv) /\
+  config_pre a /\ (
   match i with
   | Vale_AES128
   | Vale_AES256 ->
-      EverCrypt.TargetConfig.x64 /\
-      Vale.X64.CPU_Features_s.(aesni_enabled /\ pclmulqdq_enabled /\ avx_enabled /\ movbe_enabled /\ sse_enabled) /\
       // Expanded key length + precomputed stuff + scratch space (AES-GCM specific)
       B.length ek =
         vale_xkey_length (cipher_alg_of_supported_alg a) + 176
@@ -159,60 +158,41 @@ let create_in #a r dst k =
 #push-options "--z3rlimit 10 --max_fuel 0 --max_ifuel 0 --z3cliopt smt.QI.EAGER_THRESHOLD=5"
 
 let create_in_stack_chacha20_poly1305: create_in_stack_ty CHACHA20_POLY1305 =
-  fun dst k ->
+  fun k ->
   let h0 = ST.get () in
   let ek = B.alloca 0uy 32ul in
-  let h1 = ST.get () in
   let p = B.alloca (Ek Hacl_CHACHA20 (G.hide (B.as_seq h0 k)) ek) 1ul in
-  let h2 = ST.get () in
   B.blit k 0ul ek 0ul 32ul;
-  B.upd dst 0ul p;
   let h3 = ST.get() in
-  B.modifies_only_not_unused_in B.(loc_buffer dst) h0 h3;
-  Success
+  B.modifies_only_not_unused_in B.loc_none h0 h3;
+  p
 
 #pop-options
 
 inline_for_extraction noextract
 let create_in_stack_aes_gcm (i: vale_impl):
   create_in_stack_ty (alg_of_vale_impl i) =
-fun dst k ->
+  fun k ->
   let a = alg_of_vale_impl i in
   let h0 = ST.get () in
   let kv: G.erased (kv a) = G.hide (B.as_seq h0 k) in
-  let has_aesni = EverCrypt.AutoConfig2.has_aesni () in
-  let has_pclmulqdq = EverCrypt.AutoConfig2.has_pclmulqdq () in
-  let has_avx = EverCrypt.AutoConfig2.has_avx() in
-  let has_sse = EverCrypt.AutoConfig2.has_sse() in
-  let has_movbe = EverCrypt.AutoConfig2.has_movbe() in
-  if EverCrypt.TargetConfig.x64 && (has_aesni && has_pclmulqdq && has_avx && has_sse && has_movbe) then (
-    let ek = B.alloca 0uy (concrete_xkey_len i + 176ul) in
-
-    vale_expand i k ek;
-
-    let h2 = ST.get () in
-    B.modifies_only_not_unused_in B.loc_none h0 h2;
-    let p = B.alloca (Ek i (G.hide (B.as_seq h0 k)) ek) 1ul in
-    let open LowStar.BufferOps in
-    dst *= p;
-    let h3 = ST.get() in
-    B.modifies_only_not_unused_in B.(loc_buffer dst) h2 h3;
-    Success
-
-  ) else
-    UnsupportedAlgorithm
+  let ek = B.alloca 0uy (concrete_xkey_len i + 176ul) in
+  vale_expand i k ek;
+  let h2 = ST.get () in
+  B.modifies_only_not_unused_in B.loc_none h0 h2;
+  let p = B.alloca (Ek i (G.hide (B.as_seq h0 k)) ek) 1ul in
+  p
 
 let create_in_stack_aes128_gcm: create_in_stack_ty AES128_GCM =
   create_in_stack_aes_gcm Vale_AES128
 let create_in_stack_aes256_gcm: create_in_stack_ty AES256_GCM =
   create_in_stack_aes_gcm Vale_AES256
 
-let create_in_stack #a dst k =
+let create_in_stack #a k =
   match a with
-  | AES128_GCM -> create_in_stack_aes128_gcm dst k
-  | AES256_GCM -> create_in_stack_aes256_gcm dst k
-  | CHACHA20_POLY1305 -> create_in_stack_chacha20_poly1305 dst k
-  | _ -> UnsupportedAlgorithm
+  | AES128_GCM -> create_in_stack_aes128_gcm k
+  | AES256_GCM -> create_in_stack_aes256_gcm k
+  | CHACHA20_POLY1305 -> create_in_stack_chacha20_poly1305 k
 
 inline_for_extraction noextract
 let aes_gcm_encrypt (i: vale_impl):
